src/Lean/Elab/Tactic/Grind.lean
@@ -197,14 +197,16 @@ private def mkGrindOnly
         else
           let decl : Ident := mkIdent (← unresolveNameGlobalAvoidingLocals declName)
           let param ← match kind with
-            | .eqLhs   => `(Parser.Tactic.grindParam| = $decl)
-            | .eqRhs   => `(Parser.Tactic.grindParam| =_ $decl)
-            | .eqBoth  => `(Parser.Tactic.grindParam| _=_ $decl)
-            | .eqBwd   => `(Parser.Tactic.grindParam| ←= $decl)
-            | .bwd     => `(Parser.Tactic.grindParam| ← $decl)
-            | .fwd     => `(Parser.Tactic.grindParam| → $decl)
-            | .user    => `(Parser.Tactic.grindParam| usr $decl)
-            | .default => `(Parser.Tactic.grindParam| $decl:ident)
+            | .eqLhs     => `(Parser.Tactic.grindParam| = $decl)
+            | .eqRhs     => `(Parser.Tactic.grindParam| =_ $decl)
+            | .eqBoth    => `(Parser.Tactic.grindParam| _=_ $decl)
+            | .eqBwd     => `(Parser.Tactic.grindParam| ←= $decl)
+            | .bwd       => `(Parser.Tactic.grindParam| ← $decl)
+            | .fwd       => `(Parser.Tactic.grindParam| → $decl)
+            | .leftRight => `(Parser.Tactic.grindParam| => $decl)
+            | .rightLeft => `(Parser.Tactic.grindParam| <= $decl)
+            | .user      => `(Parser.Tactic.grindParam| usr $decl)
+            | .default   => `(Parser.Tactic.grindParam| $decl:ident)
           params := params.push param
   for declName in trace.eagerCases.toList do
     unless Grind.isBuiltinEagerCases declName do
