tests/lean/run/no_grind_constProp.lean
@@ -1,0 +1,508 @@
+set_option profiler true
+
+abbrev Var := String
+
+inductive Val where
+  | int  (i : Int)
+  | bool (b : Bool)
+  deriving DecidableEq, Repr
+
+instance : Coe Bool Val where
+  coe b := .bool b
+
+instance : OfNat Val n where
+  ofNat := .int n
+
+inductive BinOp where
+  | eq | and | lt | add | sub
+  deriving Repr
+
+inductive UnaryOp where
+  | not
+  deriving Repr
+
+inductive Expr where
+  | val (v : Val)
+  | var (x : Var)
+  | bin (lhs : Expr) (op : BinOp) (rhs : Expr)
+  | una (op : UnaryOp) (arg : Expr)
+  deriving Repr
+
+@[simp] def BinOp.eval : BinOp → Val → Val → Option Val
+  | .eq,  v₁,        v₂      => some (.bool (v₁ = v₂))
+  | .and, .bool b₁, .bool b₂ => some (.bool (b₁ && b₂))
+  | .lt,  .int i₁,  .int i₂  => some (.bool (i₁ < i₂))
+  | .add, .int i₁,  .int i₂  => some (.int (i₁ + i₂))
+  | .sub, .int i₁,  .int i₂  => some (.int (i₁ - i₂))
+  | _,    _,        _        => none
+
+@[simp] def UnaryOp.eval : UnaryOp → Val → Option Val
+  | .not, .bool b => some (.bool !b)
+  | _,    _       => none
+
+inductive Stmt where
+  | skip
+  | assign (x : Var) (e : Expr)
+  | seq    (s₁ s₂ : Stmt)
+  | ite    (c : Expr) (e t : Stmt)
+  | while  (c : Expr) (b : Stmt)
+  deriving Repr
+
+infix:150 " ::= " => Stmt.assign
+infixr:130 ";; "   => Stmt.seq
+
+abbrev State := List (Var × Val)
+
+@[simp] def State.update (σ : State) (x : Var) (v : Val) : State :=
+  match σ with
+  | [] => [(x, v)]
+  | (y, w)::σ => if x = y then (x, v)::σ else (y, w) :: update σ x v
+
+@[simp] def State.find? (σ : State) (x : Var) : Option Val :=
+  match σ with
+  | [] => none
+  | (y, v) :: σ => if x = y then some v else find? σ x
+
+def State.get (σ : State) (x : Var) : Val :=
+  σ.find? x |>.getD (.int 0)
+
+@[simp] def State.erase (σ : State) (x : Var) : State :=
+  match σ with
+  | [] => []
+  | (y, v) :: σ => if x = y then erase σ x else (y, v) :: erase σ x
+
+@[simp] theorem State.find?_update_self (σ : State) (x : Var) (v : Val) : (σ.update x v).find? x = some v := by
+  match σ with -- TODO: automate this proof
+  | [] => simp
+  | (y, w) :: s =>
+    simp
+    split <;> simp [*]
+    apply find?_update_self
+
+@[simp] theorem State.find?_update (σ : State) (v : Val) (h : x ≠ z) : (σ.update x v).find? z = σ.find? z := by
+  match σ with -- TODO: automate this proof
+  | [] => simp [h.symm]
+  | (y, w) :: σ =>
+    simp
+    split <;> simp [*]
+    next hc => split <;> simp_all
+    next =>
+      split
+      next => rfl
+      next => exact find?_update σ v h
+
+-- TODO: remove after we add better automation
+@[simp] theorem State.find?_update' (σ : State) (v : Val) (h : z ≠ x) : (σ.update x v).find? z = σ.find? z :=
+  State.find?_update σ v h.symm
+
+theorem State.get_of_find? {σ : State} (h : σ.find? x = some v) : σ.get x = v := by
+  simp [State.get, h, Option.getD]
+
+@[simp] theorem State.find?_erase_self (σ : State) (x : Var) : (σ.erase x).find? x = none := by
+  match σ with
+  | [] => simp
+  | (y, w) :: σ =>
+    simp
+    split <;> simp [*]
+    next => exact find?_erase_self σ y
+    next => exact find?_erase_self σ x
+
+@[simp] theorem State.find?_erase (σ : State) (h : x ≠ z) : (σ.erase x).find? z = σ.find? z := by
+  match σ with
+  | [] => simp
+  | (y, w) :: σ =>
+    simp
+    split <;> simp [*]
+    next hxy => rw [hxy] at h; simp [h.symm]; exact find?_erase σ h
+    next =>
+      split
+      next => rfl
+      next => exact find?_erase σ h
+
+-- TODO: remove after we add better automation
+@[simp] theorem State.find?_erase' (σ : State) (h : z ≠ x) : (σ.erase x).find? z = σ.find? z :=
+  State.find?_erase σ h.symm
+
+syntax ident " ↦ " term : term
+
+macro_rules
+  | `($id:ident ↦ $v:term) => `(($(Lean.quote id.getId.toString), $v:term))
+
+example : State.get [x ↦ .int 10, y ↦ .int 20] "x" = .int 10 := rfl
+
+example : State.get [x ↦ 10, y ↦ 20] "x" = 10     := rfl
+example : State.get [x ↦ 10, y ↦ true] "y" = true := rfl
+
+@[simp] def Expr.eval (σ : State) : Expr → Option Val
+  | val v   => some v
+  | var x   => σ.get x
+  | bin lhs op rhs => match lhs.eval σ, rhs.eval σ with
+    | some v₁, some v₂ => op.eval v₁ v₂  -- BinOp.eval : BinOp → Val → Val → Option Val
+    | _,       _       => none
+  | una op arg => match arg.eval σ with
+    | some v => op.eval v
+    | _      => none
+
+
+@[simp] def evalTrue  (c : Expr) (σ : State) : Prop := c.eval σ = some (Val.bool true)
+@[simp] def evalFalse (c : Expr) (σ : State) : Prop := c.eval σ = some (Val.bool false)
+
+section
+set_option hygiene false -- HACK: allow forward reference in notation
+local notation:60 "(" σ ", " s ")"  " ⇓ " σ':60 => Bigstep σ s σ'
+
+inductive Bigstep : State → Stmt → State → Prop where
+  | skip       : (σ, .skip) ⇓ σ
+  | assign     : e.eval σ = some v → (σ,  x ::= e) ⇓ σ.update x v
+  | seq        : (σ₁, s₁) ⇓ σ₂ → (σ₂, s₂) ⇓ σ₃ → (σ₁, s₁ ;; s₂) ⇓ σ₃
+  | ifTrue     : evalTrue c σ₁ → (σ₁, t) ⇓ σ₂ → (σ₁, .ite c t e) ⇓ σ₂
+  | ifFalse    : evalFalse c σ₁ → (σ₁, e) ⇓ σ₂ → (σ₁, .ite c t e) ⇓ σ₂
+  | whileTrue  : evalTrue c σ₁ → (σ₁, b) ⇓ σ₂ → (σ₂, .while c b) ⇓ σ₃ → (σ₁, .while c b) ⇓ σ₃
+  | whileFalse : evalFalse c σ → (σ, .while c b) ⇓ σ
+
+end
+
+notation:60 "(" σ ", " s ")"  " ⇓ " σ':60 => Bigstep σ s σ'
+
+/- This proof can be automated using forward reasoning. -/
+theorem Bigstem.det (h₁ : (σ, s) ⇓ σ₁) (h₂ : (σ, s) ⇓ σ₂) : σ₁ = σ₂ := by
+  induction h₁ generalizing σ₂ <;> cases h₂ <;> try simp_all
+  -- The rest of this proof should be automatic with congruence closure and a bit of forward reasoning
+  case seq ih₁ ih₂ _ h₁ h₂ =>
+    simp [ih₁ h₁] at ih₂
+    simp [ih₂ h₂]
+  case ifTrue ih h =>
+    simp [ih h]
+  case ifFalse ih h =>
+    simp [ih h]
+  case whileTrue ih₁ ih₂ h₁ h₂ =>
+    simp [ih₁ h₁] at ih₂
+    simp [ih₂ h₂]
+
+abbrev EvalM := ExceptT String (StateM State)
+
+def evalExpr (e : Expr) : EvalM Val := do
+  match e.eval (← get) with
+  | some v => return v
+  | none => throw "failed to evaluate"
+
+@[simp] def Stmt.eval (stmt : Stmt) (fuel : Nat := 100) : EvalM Unit := do
+  match fuel with
+  | 0 => throw "out of fuel"
+  | fuel+1 =>
+    match stmt with
+    | skip        => return ()
+    | assign x e  => let v ← evalExpr e; modify fun s => s.update x v
+    | seq s₁ s₂   => s₁.eval fuel; s₂.eval fuel
+    | ite c e t   =>
+      match (← evalExpr c) with
+      | .bool true  => e.eval fuel
+      | .bool false => t.eval fuel
+      | _ => throw "Boolean expected"
+    | .while c b =>
+      match (← evalExpr c) with
+      | .bool true  => b.eval fuel; stmt.eval fuel
+      | .bool false => return ()
+      | _ => throw "Boolean expected"
+
+
+@[simp] def BinOp.simplify : BinOp → Expr → Expr → Expr
+  | .eq,  .val v₁,  .val  v₂ => .val (.bool (v₁ = v₂))
+  | .and, .val (.bool a), .val (.bool b) => .val (.bool (a && b))
+  | .lt,  .val (.int a),  .val (.int b)  => .val (.bool (a < b))
+  | .add, .val (.int a), .val (.int b) => .val (.int (a + b))
+  | .sub, .val (.int a), .val (.int b) => .val (.int (a - b))
+  | op, a, b => .bin a op b
+
+@[simp] def UnaryOp.simplify : UnaryOp → Expr → Expr
+  | .not, .val (.bool b) => .val (.bool !b)
+  | op, a => .una op a
+
+@[simp] def Expr.simplify : Expr → Expr
+  | bin lhs op rhs => op.simplify lhs.simplify rhs.simplify
+  | una op arg => op.simplify arg.simplify
+  | e => e
+
+@[simp] theorem Expr.eval_simplify (e : Expr) : e.simplify.eval σ = e.eval σ := by
+  induction e with
+    -- Due to fine-grained equational theorems we have to pass `eq_def` lemmas here
+    simp only [simplify, BinOp.simplify.eq_def, eval, UnaryOp.simplify.eq_def]
+  | bin lhs op rhs ih_lhs ih_rhs =>
+    simp [← ih_lhs, ← ih_rhs]
+    split <;> simp [*]
+  | una op arg ih_arg =>
+    simp [← ih_arg]
+    split <;> simp [*]
+
+@[simp] def Stmt.simplify : Stmt → Stmt
+  | skip => skip
+  | assign x e => assign x e.simplify
+  | seq s₁ s₂ => seq s₁.simplify s₂.simplify
+  | ite c e t =>
+    match c.simplify with
+    | .val (.bool true) => e.simplify
+    | .val (.bool false) => t.simplify
+    | c' => ite c' e.simplify t.simplify
+  | .while c b =>
+    match c.simplify with
+    | .val (.bool false) => skip
+    | c' => .while c' b.simplify
+
+theorem Stmt.simplify_correct (h : (σ, s) ⇓ σ') : (σ, s.simplify) ⇓ σ' := by
+  induction h with simp_all
+  | skip => exact Bigstep.skip
+  | seq h₁ h₂ ih₁ ih₂ => exact Bigstep.seq ih₁ ih₂
+  | assign => apply Bigstep.assign; simp [*]
+  | whileTrue heq h₁ h₂ ih₁ ih₂ =>
+    rw [← Expr.eval_simplify] at heq
+    split
+    next h => rw [h] at heq; simp at heq
+    next hnp => simp [hnp] at ih₂; apply Bigstep.whileTrue heq ih₁ ih₂
+  | whileFalse heq =>
+    split
+    next => exact Bigstep.skip
+    next => apply Bigstep.whileFalse; simp [heq]
+  | ifFalse heq h ih =>
+    rw [← Expr.eval_simplify] at heq
+    split <;> simp_all
+    rw [← Expr.eval_simplify] at heq
+    apply Bigstep.ifFalse heq ih
+  | ifTrue heq h ih =>
+    rw [← Expr.eval_simplify] at heq
+    split <;> simp_all
+    rw [← Expr.eval_simplify] at heq
+    apply Bigstep.ifTrue heq ih
+
+@[simp] def Expr.constProp (e : Expr) (σ : State) : Expr :=
+  match e with
+  | val v => .val v
+  | var x => match σ.find? x with
+    | some v => val v
+    | none   => var x
+  | bin lhs op rhs => bin (lhs.constProp σ) op (rhs.constProp σ)
+  | una op arg => una op (arg.constProp σ)
+
+@[simp] theorem Expr.constProp_nil (e : Expr) : e.constProp [] = e := by
+  induction e <;> simp [*]
+
+def State.length_erase_le (σ : State) (x : Var) : (σ.erase x).length ≤ σ.length := by
+  match σ with
+  | [] => simp
+  | (y, v) :: σ =>
+    by_cases hxy : x = y <;> simp [hxy]
+    next => exact Nat.le_trans (length_erase_le σ y) (by simp_arith)
+    next => simp_arith [length_erase_le σ x]
+
+def State.length_erase_lt (σ : State) (x : Var) : (σ.erase x).length < σ.length.succ :=
+  Nat.lt_of_le_of_lt (length_erase_le ..) (by simp_arith)
+
+@[simp] def State.join (σ₁ σ₂ : State) : State :=
+  match σ₁ with
+  | [] => []
+  | (x, v) :: σ₁ =>
+    let σ₁' := erase σ₁ x -- Must remove duplicates. Alternative design: carry invariant that input state at constProp has no duplicates
+    have : (erase σ₁ x).length < σ₁.length.succ := length_erase_lt ..
+    match σ₂.find? x with
+    | some w => if v = w then (x, v) :: join σ₁' σ₂ else join σ₁' σ₂
+    | none => join σ₁' σ₂
+termination_by σ₁.length
+
+local notation "⊥" => []
+
+@[simp] def Stmt.constProp (s : Stmt) (σ : State) : Stmt × State :=
+  match s with
+  | skip => (skip, σ)
+  | assign x e => match (e.constProp σ).simplify with
+    | (.val v) => (assign x (.val v), σ.update x v)
+    | e'       => (assign x e', σ.erase x)
+  | seq s₁ s₂ => match s₁.constProp σ with
+    | (s₁', σ₁) => match s₂.constProp σ₁ with
+      | (s₂', σ₂) => (seq s₁' s₂', σ₂)
+  | ite c s₁ s₂ =>
+    match s₁.constProp σ, s₂.constProp σ with
+    | (s₁', σ₁), (s₂', σ₂) => (ite (c.constProp σ) s₁' s₂', σ₁.join σ₂)
+  | .while c b => (.while (c.constProp ⊥) (b.constProp ⊥).1, ⊥)
+
+def State.le (σ₁ σ₂ : State) : Prop :=
+  ∀ ⦃x : Var⦄ ⦃v : Val⦄, σ₁.find? x = some v → σ₂.find? x = some v
+
+infix:50 " ≼ " => State.le
+
+theorem State.le_refl (σ : State) : σ ≼ σ :=
+  fun _ _ h => h
+
+theorem State.le_trans : σ₁ ≼ σ₂ → σ₂ ≼ σ₃ → σ₁ ≼ σ₃ :=
+  fun h₁ h₂ x v h => h₂ (h₁ h)
+
+theorem State.bot_le (σ : State) : ⊥ ≼ σ :=
+  fun _ _ h => by contradiction
+
+theorem State.erase_le_cons (h : σ' ≼ σ) : σ'.erase x ≼ ((x, v) :: σ) := by
+  intro y w hf'
+  by_cases hyx : y = x <;> simp [*] at hf' |-
+  exact h hf'
+
+theorem State.cons_le_cons (h : σ' ≼ σ) : (x, v) :: σ' ≼ (x, v) :: σ := by
+  intro y w hf'
+  by_cases hyx : y = x <;> simp [*] at hf' |-
+  next => assumption
+  next => exact h hf'
+
+theorem State.cons_le_of_eq (h₁ : σ' ≼ σ) (h₂ : σ.find? x = some v) : (x, v) :: σ' ≼ σ := by
+  intro y w hf'
+  by_cases hyx : y = x <;> simp [*] at hf' |-
+  next => assumption
+  next => exact h₁ hf'
+
+theorem State.erase_le (σ : State) : σ.erase x ≼ σ := by
+  match σ with
+  | [] => simp; apply le_refl
+  | (y, v) :: σ =>
+    simp
+    split <;> try simp [*]
+    next => apply erase_le_cons; apply le_refl
+    next => apply cons_le_cons; apply erase_le
+
+theorem State.join_le_left (σ₁ σ₂ : State) : σ₁.join σ₂ ≼ σ₁ := by
+  match σ₁ with
+  | [] => simp; apply le_refl
+  | (x, v) :: σ₁ =>
+    simp
+    have : (erase σ₁ x).length < σ₁.length.succ := length_erase_lt ..
+    have ih := join_le_left (State.erase σ₁ x) σ₂
+    split
+    next y w h =>
+      split
+      next => apply cons_le_cons; apply le_trans ih (erase_le _)
+      next => apply le_trans ih (erase_le_cons (le_refl _))
+    next h => apply le_trans ih (erase_le_cons (le_refl _))
+termination_by σ₁.length
+
+theorem State.join_le_left_of (h : σ₁ ≼ σ₂) (σ₃ : State) : σ₁.join σ₃ ≼ σ₂ :=
+  le_trans (join_le_left σ₁ σ₃) h
+
+theorem State.join_le_right (σ₁ σ₂ : State) : σ₁.join σ₂ ≼ σ₂ := by
+  match σ₁ with
+  | [] => simp; apply bot_le
+  | (x, v) :: σ₁ =>
+    simp
+    have : (erase σ₁ x).length < σ₁.length.succ := length_erase_lt ..
+    have ih := join_le_right (erase σ₁ x) σ₂
+    split
+    next y w h =>
+      split <;> simp [*]
+      next => apply cons_le_of_eq ih h
+    next h => assumption
+termination_by σ₁.length
+
+theorem State.join_le_right_of (h : σ₁ ≼ σ₂) (σ₃ : State) : σ₃.join σ₁ ≼ σ₂ :=
+  le_trans (join_le_right σ₃ σ₁) h
+
+theorem State.eq_bot (h : σ ≼ ⊥) : σ = ⊥ := by
+  match σ with
+  | [] => simp
+  | (y, v) :: σ =>
+    have : State.find? ((y, v) :: σ) y = some v := by simp
+    have := h this
+    contradiction
+
+theorem State.erase_le_of_le_cons (h : σ' ≼ (x, v) :: σ) : σ'.erase x ≼ σ := by
+  intro y w hf'
+  by_cases hxy : x = y <;> simp [*] at hf'
+  have hf := h hf'
+  simp [hxy, Ne.symm hxy] at hf
+  assumption
+
+theorem State.erase_le_update (h : σ' ≼ σ) : σ'.erase x ≼ σ.update x v := by
+  intro y w hf'
+  by_cases hxy : x = y <;> simp [*] at hf' |-
+  exact h hf'
+
+theorem State.update_le_update (h : σ' ≼ σ) : σ'.update x v ≼ σ.update x v := by
+  intro y w hf
+  induction σ generalizing σ' hf with
+  | nil  => rw [eq_bot h] at hf; assumption
+  | cons zw' σ ih =>
+    have (z, w') := zw'; simp
+    have : σ'.erase z ≼ σ := erase_le_of_le_cons h
+    have ih := ih this
+    revert ih hf
+    split <;> simp [*] <;> by_cases hyz : y = z <;> simp (config := { contextual := true }) [*]
+    next =>
+      intro he'
+      have he := h he'
+      simp [*] at he
+      assumption
+    next =>
+      by_cases hxy : x = y <;> simp_all
+
+theorem Expr.eval_constProp_of_sub (e : Expr) (h : σ' ≼ σ) : (e.constProp σ').eval σ = e.eval σ := by
+  induction e with simp [*]
+  | var x =>
+    split <;> simp
+    next he => rw [State.get_of_find? (h he)]
+
+theorem Expr.eval_constProp_of_eq_of_sub {e : Expr} (h₁ : e.eval σ = v) (h₂ : σ' ≼ σ) : (e.constProp σ').eval σ = v := by
+  have := eval_constProp_of_sub e h₂
+  simp [h₁] at this
+  assumption
+
+theorem Stmt.constProp_sub (h₁ : (σ₁, s) ⇓ σ₂) (h₂ : σ₁' ≼ σ₁) : (s.constProp σ₁').2 ≼ σ₂ := by
+  induction h₁ generalizing σ₁' with simp
+  | skip => assumption
+  | assign heq =>
+    split <;> simp
+    next h =>
+      have heq' := Expr.eval_constProp_of_eq_of_sub heq h₂
+      rw [← Expr.eval_simplify, h] at heq'
+      simp at heq'
+      rw [heq']
+      apply State.update_le_update h₂
+    next h _ _ =>
+      exact State.erase_le_update h₂
+  | whileTrue heq h₃ h₄ ih₃ ih₄ =>
+    have ih₃ := ih₃ h₂
+    have ih₄ := ih₄ ih₃
+    simp [heq] at ih₄
+    exact ih₄
+  | whileFalse heq => apply State.bot_le
+  | ifTrue heq h ih =>
+    have ih := ih h₂
+    apply State.join_le_left_of ih
+  | ifFalse heq h ih =>
+    have ih := ih h₂
+    apply State.join_le_right_of ih
+  | seq h₃ h₄ ih₃ ih₄ => exact ih₄ (ih₃ h₂)
+
+theorem Stmt.constProp_correct (h₁ : (σ₁, s) ⇓ σ₂) (h₂ : σ₁' ≼ σ₁) : (σ₁, (s.constProp σ₁').1) ⇓ σ₂ := by
+  induction h₁ generalizing σ₁' with simp_all
+  | skip => exact Bigstep.skip
+  | assign heq =>
+    split <;> simp
+    next h =>
+      have heq' := Expr.eval_constProp_of_eq_of_sub heq h₂
+      rw [← Expr.eval_simplify, h] at heq'
+      simp at heq'
+      apply Bigstep.assign; simp [*]
+    next =>
+      have heq' := Expr.eval_constProp_of_eq_of_sub heq h₂
+      rw [← Expr.eval_simplify] at heq'
+      apply Bigstep.assign heq'
+  | seq h₁ h₂ ih₁ ih₂ =>
+    apply Bigstep.seq (ih₁ h₂) (ih₂ (constProp_sub h₁ h₂))
+  | whileTrue heq h₁ h₂ ih₁ ih₂ =>
+    have ih₁ := ih₁ (State.bot_le _)
+    have ih₂ := ih₂ (State.bot_le _)
+    exact Bigstep.whileTrue heq ih₁ ih₂
+  | whileFalse heq =>
+    exact Bigstep.whileFalse heq
+  | ifTrue heq h ih =>
+    exact Bigstep.ifTrue (Expr.eval_constProp_of_eq_of_sub heq h₂) (ih h₂)
+  | ifFalse heq h ih =>
+    exact Bigstep.ifFalse (Expr.eval_constProp_of_eq_of_sub heq h₂) (ih h₂)
+
+def Stmt.constPropagation (s : Stmt) : Stmt :=
+  (s.constProp ⊥).1
+
+theorem Stmt.constPropagation_correct (h : (σ, s) ⇓ σ') : (σ, s.constPropagation) ⇓ σ' :=
+  constProp_correct h (State.bot_le _)
